reflex/coq/bench-quark/PolicyTabIdUnique.v
@@ -1,0 +1,22 @@
+Require Import String.
+Require Import Reflex ReflexBase.
+Require Import PolLang ActionMatch.
+Require Import Kernel.
+
+Local Opaque str_of_string.
+
+Import SystemFeatures Language Spec.
+
+Definition Tab_pat id : conc_pat COMPT COMPS :=
+  Build_conc_pat COMPT COMPS Tab (None, (Some id, tt)).
+
+Theorem enable : forall st tr id,
+  Reach PAYD COMPT COMPTDEC COMPS KSTD IENVD INIT HANDLERS st ->
+  ktr _ _ _ _ st = inhabits tr ->
+  Disables PAYD COMPT COMPS COMPTDEC
+    (KOExec PAYD COMPT COMPS None None (Some (Tab_pat id)))
+    (KOExec PAYD COMPT COMPS None None (Some (Tab_pat id)))
+    tr.
+Proof.
+  Time solve [crush].
+Qed.
